hopefully this solves some timeout issues

Impl/StateSectorModel.i.dfy
@@ -1,19 +1,17 @@
 include "../PivotBetree/PivotBetreeSpec.i.dfy"
 include "IndirectionTableModel.i.dfy"
 include "../BlockCacheSystem/SectorType.i.dfy"
-include "../BlockCacheSystem/JournalCache.i.dfy"
 
 module StateSectorModel {
   import BT = PivotBetreeSpec`Internal
   import IndirectionTableModel
   import SectorType
-  import BC = BlockCache
-  import JC = JournalCache
 
   type Node = BT.G.Node  
+  type IndirectionTable = IndirectionTableModel.IndirectionTable
 
   datatype Sector =
     | SectorNode(node: Node)
-    | SectorIndirectionTable(indirectionTable: IndirectionTableModel.IndirectionTable)
+    | SectorIndirectionTable(indirectionTable: IndirectionTable)
     | SectorSuperblock(superblock: SectorType.Superblock)
 }
